Remove fuel for run_block, assuming termination
tests not yet updated

spec/prop/vfmExecutionPropScript.sml
@@ -1666,5 +1666,42 @@ Proof
   \\ irule_at Any decreases_gas_inc_pc_or_jump
 QED
 
-val () = export_theory();
+Definition run_tr_def:
+  run_tr (r, s) =
+    case r of INR x => (x, s)
+       | _ => run_tr (step s)
+Termination
+  cheat
+  (*
+  WF_REL_TAC`inv_image ($< LEX $<) (λp.
+    let w = contexts_weight 0 (SND p).contexts in
+    if ISR (FST p) then (0,0) else w)`
+  \\ rpt gen_tac \\ strip_tac
+  \\ mp_tac decreases_gas_step
+  \\ rewrite_tac[decreases_gas_cred_def]
+  \\ disch_then drule
+  \\ reverse(rw[LEX_DEF, UNCURRY])
+  >- metis_tac[sum_CASES, ISL, ISR]
+  \\ qmatch_goalsub_abbrev_tac`a ∨ b`
+  \\ Cases_on `a` \\ gs[Abbr`b`]
+  \\ gvs[contexts_weight_def, ok_state_def]
+  \\ Cases_on`s.contexts` \\ gs[]
+  *)
+End
 
+Theorem run_eq_tr:
+  run s = case run_tr (step s) of (x, y) => SOME (INR x, y)
+Proof
+  rw[run_def]
+  \\ rw[Once whileTheory.OWHILE_THM]
+  \\ qspec_tac(`step s`,`x`)
+  \\ Cases
+  \\ map_every qid_spec_tac [`r`,`q`]
+  \\ recInduct run_tr_ind
+  \\ rw[]
+  \\ rw[Once run_tr_def]
+  \\ CASE_TAC \\ gs[]
+  \\ rw[Once whileTheory.OWHILE_THM]
+QED
+
+val () = export_theory();
